src/opt/ReorderStore.v
@@ -74,7 +74,9 @@ Lemma sim_store_step
     (FUTURE_SRC: Memory.future mem_k_src mem1_src)
     (FUTURE_TGT: Memory.future mem_k_tgt mem1_tgt)
     (WF_SRC: Local.wf lc1_src mem1_src)
-    (WF_TGT: Local.wf lc1_tgt mem1_tgt),
+    (WF_TGT: Local.wf lc1_tgt mem1_tgt)
+    (MEM_SRC: Memory.closed mem1_src)
+    (MEM_TGT: Memory.closed mem1_tgt),
     _sim_thread_step lang lang ((sim_thread (sim_terminal eq)) \6/ sim_store)
                      st1_src lc1_src mem1_src
                      st1_tgt lc1_tgt mem1_tgt.
@@ -171,12 +173,11 @@ Proof.
     { econs 2. eauto. }
     i. des.
     + exploit program_step_promise; eauto. i.
-      punfold SIM. exploit SIM; eauto; try refl.
-      { exploit Thread.rtc_step_future; eauto. s. i. des.
-        exploit Thread.step_future; eauto. s. i. des. auto.
-      }
-      { exploit Thread.program_step_future; eauto. s. i. des. auto. }
-      i. des. exploit PROMISES; eauto. i. des.
+      exploit Thread.rtc_step_future; eauto. s. i. des.
+      exploit Thread.step_future; eauto. s. i. des.
+      exploit Thread.program_step_future; eauto. s. i. des.
+      punfold SIM. exploit SIM; eauto; try refl. s. i. des.
+      exploit PROMISES; eauto. i. des.
       eexists _, _, _. splits; [|eauto].
       etrans; eauto. etrans; [|eauto].
       econs 2; eauto. econs; eauto. etrans; eauto.
